Partially flesh out [freeze] proofs; also parameterize [sqrt_5mod8] over implementations of [mul] and [pow] so bounds can be threaded through

src/ModularArithmetic/ModularBaseSystem.v
@@ -77,15 +77,17 @@ Section ModularBaseSystem.
   (* Note : both of the following square root definitions will produce garbage output if the input is
             not square mod [modulus]. The caller should either provably only call them with square input,
             or test that the output squared is in fact equal to the input and case split. *)
-  Definition sqrt_5mod8 (chain : list (nat * nat))
-                  (chain_correct : fold_chain 0%N N.add chain (1%N :: nil) = Z.to_N (modulus / 8 + 1))
-                  (sqrt_minus1 x : digits) : digits :=
-    let b := pow x chain in if eqb (mul b b) x then b else mul sqrt_minus1 b.
-
   Definition sqrt_3mod4 (chain : list (nat * nat))
                   (chain_correct : fold_chain 0%N N.add chain (1%N :: nil) = Z.to_N (modulus / 4 + 1))
                   (x : digits) : digits := pow x chain.
 
+  (* sqrt_5mod8 is parameterized over implementation of [mul] and [pow] because it relies on bounds-checking
+     for these two functions, which is much easier for simplified implementations than the more generalized
+     ones defined here. *)
+  Definition sqrt_5mod8 mul_ pow_ (chain : list (nat * nat))
+                  (chain_correct : fold_chain 0%N N.add chain (1%N :: nil) = Z.to_N (modulus / 8 + 1))
+                  (sqrt_minus1 x : digits) : digits :=
+    let b := pow_ x chain in if eqb (mul_ b b) x then b else mul_ sqrt_minus1 b.
 
   Import Morphisms.
   Global Instance eq_Equivalence : Equivalence eq.
