src/ModularArithmetic/ModularBaseSystemProofs.v
@@ -177,6 +177,19 @@ Section FieldOperationProofs.
     pose proof prime_modulus; prime_bound.
   Qed.
 
+  Lemma encode_range : forall x,
+    0 <= BaseSystem.decode base (to_list (encode x)) < modulus.
+  Proof.
+    cbv [encode]; intros.
+    rewrite to_list_from_list.
+    rewrite encode_eq.
+    rewrite BaseSystemProofs.encode_rep; auto using F.to_Z_range, modulus_pos, bv.
+    + pose proof (F.to_Z_range x modulus_pos).
+      replace (2 ^ k) with (modulus + c) by (cbv[c]; ring).
+      pose proof c_pos; omega.
+    + apply base_upper_bound_compatible; auto.
+  Qed.
+
   Lemma add_rep : forall u v x y, u ~= x -> v ~= y ->
     add u v ~= (x+y)%F.
   Proof.
@@ -521,6 +534,17 @@ Section CarryProofs.
   Qed.
   Hint Resolve carry_rep.
 
+  Lemma decode_mod_Fdecode : forall u, length u = length limb_widths ->
+    BaseSystem.decode base u mod modulus= F.to_Z (decode (from_list_default 0 _ u)).
+  Proof.
+    intros.
+    rewrite <-(to_list_from_list _ u) with (pf := H).
+    erewrite Fdecode_decode_mod by reflexivity.
+    rewrite to_list_from_list.
+    rewrite from_list_default_eq with (pf := H).
+    reflexivity.
+  Qed.
+
   Lemma carry_sequence_rep : forall is us x,
     (forall i, In i is -> (i < length limb_widths)%nat) ->
     us ~= x -> forall pf, from_list _ (carry_sequence is (to_list _ us)) pf ~= x.
@@ -849,26 +873,62 @@ Section CanonicalizationProofs.
       auto using length_carry_full, bound_after_second_loop.
   Qed.
 
-  (* TODO(jadep):
-     - Proof of correctness for [ge_modulus] and [cond_subtract_modulus]
-     - Proof of correctness for [freeze]
-       * freeze us = encode (decode us)
-       * decode us = x ->
-         canonicalized_BSToWord (freeze us)) = FToWord x
+  Lemma ge_modulus_spec : forall u, length u = length limb_widths ->
+    (ge_modulus u = false <-> 0 <= BaseSystem.decode base u < modulus).
+  Proof.
+  Admitted.
 
-         (where [canonicalized_BSToWord] uses bitwise operations to concatenate digits
-          in BaseSystem in canonical form, splitting along word capacities)
-  *)
+  Lemma conditional_subtract_modulus_spec : forall u cond,
+    length u = length limb_widths ->
+    BaseSystem.decode base (conditional_subtract_modulus u cond) =
+    BaseSystem.decode base u - (if cond then 1 else 0) * modulus.
+  Proof.
+  Admitted.
+
+  Lemma conditional_subtract_modulus_preserves_bounded : forall u,
+      bounded limb_widths u ->
+      bounded limb_widths (conditional_subtract_modulus u (ge_modulus u)).
+  Proof.
+  Admitted.
+
+  Lemma conditional_subtract_lt_modulus : forall u,
+    bounded limb_widths u ->
+    ge_modulus (conditional_subtract_modulus u (ge_modulus u)) = false.
+  Proof.
+  Admitted.
 
   (* bounded canonical -> freeze bounded -> freeze canonical *)
 
-      Import SetoidList.
+  Import SetoidList.
   (* TODO : move to Tuple *)
   Lemma fieldwise_to_list_iff : forall {T n} R (s t : tuple T n),
-    (fieldwise R s t <-> Forall2 R (to_list _ s) (to_list _ t)).
-  Admitted.
+      (fieldwise R s t <-> Forall2 R (to_list _ s) (to_list _ t)).
+  Proof.
+    induction n; split; intros.
+    + constructor.
+    + cbv [fieldwise]. auto.
+    + destruct n; cbv [tuple to_list fieldwise] in *.
+      - cbv [to_list']; auto.
+      - simpl in *. destruct s,t; cbv [fst snd] in *.
+        constructor; intuition auto.
+        apply IHn; auto.
+    + destruct n; cbv [tuple to_list fieldwise] in *.
+      - cbv [fieldwise']; auto.
+        cbv [to_list'] in *; inversion H; auto.
+      - simpl in *. destruct s,t; cbv [fst snd] in *.
+        inversion H; subst.
+        split; try assumption.
+        apply IHn; auto.
+  Qed.
   
-  (* convenience notation -- [bounded] for digits rather than lists *)
+
+  Local Notation initial_bounds u := 
+      (forall n : nat,
+       0 <= to_list (length limb_widths) u [n] <
+       2 ^ B -
+       (if PeanoNat.Nat.eq_dec n 0
+        then 0
+        else (2 ^ B) >> (limb_widths [Init.Nat.pred n]))).
   Local Notation minimal_rep u := ((bounded limb_widths (to_list (length limb_widths) u))
                                    /\ (ge_modulus (to_list _ u) = false)).
   Import Morphisms.
@@ -920,12 +980,11 @@ Section CanonicalizationProofs.
   Qed.
 
   Lemma minimal_rep_encode : forall x, minimal_rep (encode x).
-  Admitted.
-
-  Lemma ge_modulus_spec : forall u, length u = length limb_widths ->
-                                    ge_modulus u = false ->
-                                    0 <= BaseSystem.decode base u < modulus.
-  Admitted.
+  Proof.
+    split; intros; auto using bounded_encode.
+    apply ge_modulus_spec; auto using length_to_list.
+    apply encode_range.
+  Qed.
 
   Lemma encode_minimal_rep : forall u x, rep u x -> minimal_rep u ->
                                          fieldwise Logic.eq u (encode x).
@@ -958,14 +1017,64 @@ Section CanonicalizationProofs.
       congruence.
   Qed.
 
-  Lemma minimal_rep_freeze : forall u, minimal_rep (freeze u).
-  Admitted.
+  Lemma minimal_rep_freeze : forall u, initial_bounds u ->
+      minimal_rep (freeze u).
+  Proof.
+    repeat match goal with
+           | |- _ => progress (cbv [freeze ModularBaseSystemList.freeze])
+           | |- _ => progress intros
+           | |- minimal_rep _ => split
+           | |- _ => rewrite to_list_from_list
+           | |- _ => apply bound_after_third_loop
+           | |- _ => apply conditional_subtract_lt_modulus
+           | |- _ => apply conditional_subtract_modulus_preserves_bounded
+           | |- bounded _ (carry_full _) => apply bounded_iff
+           | |- _ => solve [auto using length_to_list]
+           end.
+  Qed.
+
+  Lemma freeze_decode : forall u,
+      BaseSystem.decode base (to_list _ (freeze u)) mod modulus =
+      BaseSystem.decode base (to_list _ u) mod modulus.
+  Proof.
+    repeat match goal with
+           | |- _ => progress cbv [freeze ModularBaseSystemList.freeze]
+           | |- _ => progress intros
+           | |- _ => rewrite <-Z.add_opp_r, <-Z.mul_opp_l
+           | |- _ => rewrite Z.mod_add by (pose proof prime_modulus; prime_bound)
+           | |- _ => rewrite to_list_from_list
+           | |- _ => rewrite conditional_subtract_modulus_spec by
+                       auto using length_carry_full, length_to_list
+           end.
+    rewrite !decode_mod_Fdecode by auto using length_carry_full, length_to_list.
+    cbv [carry_full].
+    apply F.eq_to_Z_iff.
+    rewrite <-@to_list_from_list with (pf := length_carry_sequence (length_carry_sequence (length_to_list _))).
+    rewrite from_list_default_eq with (pf := length_carry_sequence (length_to_list _)).
+    rewrite carry_sequence_rep; try reflexivity; try apply make_chain_lt.
+    cbv [rep].
+    rewrite <-from_list_default_eq with (d := 0).
+    erewrite <-to_list_from_list with (pf := length_carry_sequence (length_to_list _)).
+    rewrite from_list_default_eq with (pf := length_carry_sequence (length_to_list _)).
+    rewrite carry_sequence_rep; try reflexivity; try apply make_chain_lt.
+    cbv [rep].
+    rewrite carry_sequence_rep; try reflexivity; try apply make_chain_lt.
+    rewrite from_list_default_eq with (pf := length_to_list _).
+    rewrite from_list_to_list; reflexivity.
+  Qed.
 
   Lemma freeze_rep : forall u x, rep u x -> rep (freeze u) x.
-  Admitted.
+  Proof.
+    cbv [rep]; intros.
+    apply F.eq_to_Z_iff.
+    erewrite <-!Fdecode_decode_mod by eauto.
+    apply freeze_decode.
+  Qed.
   
   Lemma freeze_canonical : forall u v x y, rep u x -> rep v y ->
-                                           (x = y <-> fieldwise Logic.eq (freeze u) (freeze v)).
+                                           initial_bounds u ->
+                                           initial_bounds v ->
+    (x = y <-> fieldwise Logic.eq (freeze u) (freeze v)).
   Proof.
     intros; apply bounded_canonical; auto using freeze_rep, minimal_rep_freeze.
   Qed.
@@ -979,12 +1088,35 @@ Section SquareRootProofs.
   Local Notation base := (base_from_limb_widths limb_widths).
   Local Hint Resolve (@limb_widths_nonneg _ prm) sum_firstn_limb_widths_nonneg.
 
-  Lemma eqb_correct : forall u v x y, u ~= x -> v ~= y ->
-                                      (x = y <-> eqb u v = true).
+  Definition freeze_input_bounds n := 
+     (2 ^ B -
+       (if PeanoNat.Nat.eq_dec n 0
+        then 0
+        else (2 ^ B) >> (nth_default 0 limb_widths (Init.Nat.pred n)))).
+  Definition bounded_by u bounds := 
+      (forall n : nat,
+          0 <= nth_default 0 (to_list (length limb_widths) u) n < bounds n).
+  
+  Lemma eqb_true_iff : forall u v x y,
+    bounded_by u freeze_input_bounds -> bounded_by v freeze_input_bounds ->
+    u ~= x -> v ~= y -> (x = y <-> eqb u v = true).
   Proof.
-    cbv [eqb]. intros.
+    cbv [eqb freeze_input_bounds]. intros.
     rewrite fieldwiseb_fieldwise by (apply Z.eqb_eq).
     eauto using freeze_canonical.
+  Qed.
+
+  Lemma eqb_false_iff : forall u v x y,
+    bounded_by u freeze_input_bounds -> bounded_by v freeze_input_bounds ->
+    u ~= x -> v ~= y -> (x <> y <-> eqb u v = false).
+  Proof.
+    intros.
+    case_eq (eqb u v).
+    + rewrite <-eqb_true_iff by eassumption; intros; split; congruence.
+    + split; intros; auto.
+      intro Hfalse_eq;
+        rewrite (eqb_true_iff u v) in Hfalse_eq by eassumption.
+      congruence.
   Qed.
 
   Section Sqrt3mod4.
@@ -1007,9 +1139,21 @@ Section SquareRootProofs.
   Context (modulus_5mod8 : modulus mod 8 = 5).
   Context {ec : ExponentiationChain (modulus / 8 + 1)}.
   Context (sqrt_m1 : digits) (sqrt_m1_correct : mul sqrt_m1 sqrt_m1 ~= F.opp 1%F).
+  Context (mul_ : digits -> digits -> digits)
+          (mul_equiv : forall x y, mul_ x y = mul x y)
+          {mul_input_bounds : nat -> Z}
+          (mul_bounded : forall x y, bounded_by x mul_input_bounds ->
+                                     bounded_by y mul_input_bounds ->
+                                     bounded_by (mul_ x y) freeze_input_bounds).
+  Context (pow_ : digits -> list (nat * nat) -> digits)
+          (pow_equiv : forall x is, pow_ x is = pow x is)
+          {pow_input_bounds : nat -> Z}
+          (pow_bounded : forall x is, bounded_by x pow_input_bounds ->
+                                      bounded_by (pow_ x is) mul_input_bounds).
   
   Lemma sqrt_5mod8_correct : forall u x, u ~= x ->
-    (sqrt_5mod8 chain chain_correct sqrt_m1 u) ~= F.sqrt_5mod8 (decode sqrt_m1) x.
+    bounded_by u pow_input_bounds -> bounded_by u freeze_input_bounds ->
+    (sqrt_5mod8 mul_ pow_ chain chain_correct sqrt_m1 u) ~= F.sqrt_5mod8 (decode sqrt_m1) x.
   Proof.
     repeat match goal with
            | |- _ => progress (cbv [sqrt_5mod8 F.sqrt_5mod8]; intros)
@@ -1017,9 +1161,19 @@ Section SquareRootProofs.
            | |- _ => rewrite eqb_correct in * by eassumption
            | |- (if eqb ?a ?b then _ else _) ~=
                 (if dec (?c = _) then _ else _) =>
-             assert (a ~= c); repeat break_if; try apply mul_rep;
-               try solve [rewrite <-chain_correct; apply pow_rep; eassumption]
-           | |- _ => congruence
+               assert (a ~= c); rewrite !mul_equiv, pow_equiv in *;
+               repeat break_if
+           | |- _ => apply mul_rep; try reflexivity;
+                       rewrite <-chain_correct; apply pow_rep; eassumption
+           | |- _ => rewrite <-chain_correct;  apply pow_rep; eassumption
+           | H : eqb ?a ?b = true |- _ =>
+             rewrite <-(eqb_true_iff a b) in Heqb
+               by (eassumption || rewrite <-mul_equiv, <-pow_equiv;
+                     apply mul_bounded, pow_bounded; auto); congruence
+           | H : eqb ?a ?b = false |- _ =>
+             rewrite <-(eqb_false_iff a b) in Heqb
+               by (eassumption || rewrite <-mul_equiv, <-pow_equiv;
+                     apply mul_bounded, pow_bounded; auto); congruence
            end.
   Qed.
   End Sqrt5mod8.
